<?xml version="1.0"?>
<rdf:RDF xmlns="http://www.owl-ontologies.com/Ontology1482491841.owl#"
     xml:base="http://www.owl-ontologies.com/Ontology1482491841.owl"
     xmlns:p1="http://purl.org/dc/elements/1.1#"
     xmlns:ns="http://www.w3.org/2003/06/sw-vocab-status/ns#"
     xmlns:owl="http://www.w3.org/2002/07/owl#"
     xmlns:swrlb="http://www.w3.org/2003/11/swrlb#"
     xmlns:protege="http://protege.stanford.edu/plugins/owl/protege#"
     xmlns:swrl="http://www.w3.org/2003/11/swrl#"
     xmlns:xsd="http://www.w3.org/2001/XMLSchema#"
     xmlns:skos="http://www.w3.org/2004/02/skos/core#"
     xmlns:rdfs="http://www.w3.org/2000/01/rdf-schema#"
     xmlns:vcard="http://www.w3.org/2006/vcard/ns#"
     xmlns:xsp="http://www.owl-ontologies.com/2005/08/07/xsp.owl#"
     xmlns:rdf="http://www.w3.org/1999/02/22-rdf-syntax-ns#"
     xmlns:terms="http://purl.org/dc/terms/"
     xmlns:xml="http://www.w3.org/XML/1998/namespace"
     xmlns:wot="http://xmlns.com/wot/0.1/"
     xmlns:foaf="http://xmlns.com/foaf/0.1/"
     xmlns:dc="http://purl.org/dc/elements/1.1/">
    <owl:Ontology rdf:about="http://www.owl-ontologies.com/Ontology1482491841.owl">
        <owl:imports rdf:resource="http://www.w3.org/2006/vcard/ns"/>
        <owl:imports rdf:resource="http://www.w3.org/2000/01/rdf-schema#"/>
        <owl:imports rdf:resource="http://xmlns.com/foaf/0.1/"/>
    </owl:Ontology>
    


    <!-- 
    ///////////////////////////////////////////////////////////////////////////////////////
    //
    // Annotation properties
    //
    ///////////////////////////////////////////////////////////////////////////////////////
     -->

    


    <!-- http://purl.org/dc/terms/description -->

    <owl:AnnotationProperty rdf:about="http://purl.org/dc/terms/description"/>
    


    <!-- http://purl.org/dc/terms/hasVersion -->

    <owl:AnnotationProperty rdf:about="http://purl.org/dc/terms/hasVersion"/>
    


    <!-- http://purl.org/dc/terms/issued -->

    <owl:AnnotationProperty rdf:about="http://purl.org/dc/terms/issued"/>
    


    <!-- http://purl.org/dc/terms/modified -->

    <owl:AnnotationProperty rdf:about="http://purl.org/dc/terms/modified"/>
    


    <!-- http://purl.org/dc/terms/publisher -->

    <owl:AnnotationProperty rdf:about="http://purl.org/dc/terms/publisher"/>
    


    <!-- http://purl.org/dc/terms/title -->

    <owl:AnnotationProperty rdf:about="http://purl.org/dc/terms/title"/>
    


    <!-- http://www.w3.org/2004/02/skos/core#note -->

    <owl:AnnotationProperty rdf:about="http://www.w3.org/2004/02/skos/core#note"/>
    


    <!-- 
    ///////////////////////////////////////////////////////////////////////////////////////
    //
    // Datatypes
    //
    ///////////////////////////////////////////////////////////////////////////////////////
     -->

    


    <!-- http://www.w3.org/2000/01/rdf-schema#Resource -->

    <rdfs:Datatype rdf:about="http://www.w3.org/2000/01/rdf-schema#Resource"/>
    


    <!-- http://www.w3.org/2001/XMLSchema#date -->

    <rdfs:Datatype rdf:about="http://www.w3.org/2001/XMLSchema#date"/>
    


    <!-- 
    ///////////////////////////////////////////////////////////////////////////////////////
    //
    // Object Properties
    //
    ///////////////////////////////////////////////////////////////////////////////////////
     -->

    


    <!-- http://www.owl-ontologies.com/Ontology1482491841.owl#LearningOpportunityInstance -->

    <owl:ObjectProperty rdf:about="http://www.owl-ontologies.com/Ontology1482491841.owl#LearningOpportunityInstance">
        <rdfs:range rdf:resource="http://www.owl-ontologies.com/Ontology1482491841.owl#LearningOpportunityInstance"/>
    </owl:ObjectProperty>
    


    <!-- http://www.owl-ontologies.com/Ontology1482491841.owl#hasPart -->

    <owl:ObjectProperty rdf:about="http://www.owl-ontologies.com/Ontology1482491841.owl#hasPart">
        <rdfs:subPropertyOf rdf:resource="http://www.owl-ontologies.com/Ontology1482491841.owl#LearningOpportunityInstance"/>
        <rdfs:domain rdf:resource="http://www.owl-ontologies.com/Ontology1482491841.owl#LearningOpportunityObject"/>
        <rdfs:range rdf:resource="http://www.owl-ontologies.com/Ontology1482491841.owl#LearningOpportunityObject"/>
        <rdfs:comment>Definition: A relation to a Learning Opportunity Object that is logically included in the Learning Opportunity
Object.
Comments: This can be used to represent part-whole relations, such as the relationship between
organisations and departments, or between programmes and constituent units. Content should be
a URI conforming to IETF\-RFC2396. Attention is drawn to the property
http://purl.org/dc/terms/hasPart as defined by DCMI\-TERMS as an equivalent property.</rdfs:comment>
        <rdfs:label>Has part</rdfs:label>
    </owl:ObjectProperty>
    


    <!-- http://www.owl-ontologies.com/Ontology1482491841.owl#offeredAt -->

    <owl:ObjectProperty rdf:about="http://www.owl-ontologies.com/Ontology1482491841.owl#offeredAt">
        <rdfs:subPropertyOf rdf:resource="http://www.owl-ontologies.com/Ontology1482491841.owl#LearningOpportunityInstance"/>
        <rdfs:domain rdf:resource="http://www.owl-ontologies.com/Ontology1482491841.owl#LearningOpportunityInstance"/>
        <rdfs:range rdf:resource="http://www.owl-ontologies.com/Ontology1482491841.owl#LearningOpportunityProvider"/>
        <rdfs:comment>Definition: A relation to a Learning Opportunity Provider that offers the Learning Opportunity Instance.
Comments: This can be used to represent franchises or other circumstances when the provider that offers
the instance is different to the provider that defines the specification. Content should be a URI
conforming to IETF\-RFC2396.</rdfs:comment>
        <rdfs:label>Offered At</rdfs:label>
    </owl:ObjectProperty>
    


    <!-- http://www.owl-ontologies.com/Ontology1482491841.owl#offers -->

    <owl:ObjectProperty rdf:about="http://www.owl-ontologies.com/Ontology1482491841.owl#offers">
        <rdfs:subPropertyOf rdf:resource="http://www.owl-ontologies.com/Ontology1482491841.owl#LearningOpportunityInstance"/>
        <rdfs:domain rdf:resource="http://www.owl-ontologies.com/Ontology1482491841.owl#LearningOpportunityProvider"/>
        <rdfs:range rdf:resource="http://www.owl-ontologies.com/Ontology1482491841.owl#LearningOpportunitySpecification"/>
        <rdfs:comment>Definition: A relation to a Learning Opportunity Specification offered by the Learning Opportunity Provider.
Comments: Content should be a URI conforming to IETF\-RFC2396.</rdfs:comment>
        <rdfs:label>Offers</rdfs:label>
    </owl:ObjectProperty>
    


    <!-- http://www.owl-ontologies.com/Ontology1482491841.owl#specifies -->

    <owl:ObjectProperty rdf:about="http://www.owl-ontologies.com/Ontology1482491841.owl#specifies">
        <rdfs:subPropertyOf rdf:resource="http://www.owl-ontologies.com/Ontology1482491841.owl#LearningOpportunityInstance"/>
        <rdfs:domain rdf:resource="http://www.owl-ontologies.com/Ontology1482491841.owl#LearningOpportunitySpecification"/>
        <rdfs:range rdf:resource="http://www.owl-ontologies.com/Ontology1482491841.owl#LearningOpportunityInstance"/>
        <rdfs:comment>Definition: A relation to a Learning Opportunity Instance that is an instance specified by the Learning
Opportunity Specification.
Comments: Content should be a URI conforming to IETF\-RFC2396</rdfs:comment>
        <rdfs:label>Specifies</rdfs:label>
    </owl:ObjectProperty>
    


    <!-- 
    ///////////////////////////////////////////////////////////////////////////////////////
    //
    // Data properties
    //
    ///////////////////////////////////////////////////////////////////////////////////////
     -->

    


    <!-- http://purl.org/dc/elements/1.1/date -->

    <owl:DatatypeProperty rdf:about="http://purl.org/dc/elements/1.1/date">
        <terms:description xml:lang="en">Date may be used to express temporal information at any level of granularity.  Recommended best practice is to use an encoding scheme, such as the W3CDTF profile of ISO 8601 [W3CDTF].</terms:description>
        <terms:hasVersion rdf:resource="http://dublincore.org/usage/terms/history/#date-006"/>
        <terms:issued rdf:datatype="http://www.w3.org/2001/XMLSchema#date">1999-07-02</terms:issued>
        <terms:modified rdf:datatype="http://www.w3.org/2001/XMLSchema#date">2008-01-14</terms:modified>
        <rdfs:comment xml:lang="en">A point or period of time associated with an event in the lifecycle of the resource.</rdfs:comment>
        <rdfs:isDefinedBy rdf:resource="http://purl.org/dc/elements/1.1/"/>
        <rdfs:label xml:lang="en">Date</rdfs:label>
        <skos:note xml:lang="en">A second property with the same name as this property has been declared in the dcterms: namespace (http://purl.org/dc/terms/).  See the Introduction to the document &quot;DCMI Metadata Terms&quot; (http://dublincore.org/documents/dcmi-terms/) for an explanation.</skos:note>
    </owl:DatatypeProperty>
    


    <!-- http://www.owl-ontologies.com/Ontology1482491841.owl#assessment -->

    <owl:DatatypeProperty rdf:about="http://www.owl-ontologies.com/Ontology1482491841.owl#assessment">
        <rdfs:domain rdf:resource="http://www.owl-ontologies.com/Ontology1482491841.owl#LearningOpportunityInstance"/>
        <rdfs:range rdf:resource="http://www.w3.org/2000/01/rdf-schema#Resource"/>
        <rdfs:comment>Definition: assessment strategy: a description of the broad approach to assessment used in the learning
opportunity.
Comments: Examples include types of assessments and evaluations of learning and competency
development such as exams, mostly by coursework etc.</rdfs:comment>
        <rdfs:label>Assessment</rdfs:label>
    </owl:DatatypeProperty>
    


    <!-- http://www.owl-ontologies.com/Ontology1482491841.owl#cost -->

    <owl:DatatypeProperty rdf:about="http://www.owl-ontologies.com/Ontology1482491841.owl#cost">
        <rdfs:domain rdf:resource="http://www.owl-ontologies.com/Ontology1482491841.owl#LearningOpportunityInstance"/>
        <rdfs:range rdf:resource="http://www.w3.org/2000/01/rdf-schema#Literal"/>
        <rdfs:comment>Definition: A cost associated with obtaining access to the Learning Opportunity Instance.
Comments:</rdfs:comment>
        <rdfs:label>Cost</rdfs:label>
    </owl:DatatypeProperty>
    


    <!-- http://www.owl-ontologies.com/Ontology1482491841.owl#credit -->

    <owl:DatatypeProperty rdf:about="http://www.owl-ontologies.com/Ontology1482491841.owl#credit">
        <rdfs:domain rdf:resource="http://www.owl-ontologies.com/Ontology1482491841.owl#LearningOpportunitySpecification"/>
        <rdfs:range rdf:resource="http://www.w3.org/2000/01/rdf-schema#Resource"/>
        <rdfs:comment>Definition: An account of the credits that can be obtained from completion of a Learning Opportunity.</rdfs:comment>
        <rdfs:label>Credit</rdfs:label>
    </owl:DatatypeProperty>
    


    <!-- http://www.owl-ontologies.com/Ontology1482491841.owl#duration -->

    <owl:DatatypeProperty rdf:about="http://www.owl-ontologies.com/Ontology1482491841.owl#duration">
        <rdfs:subPropertyOf rdf:resource="http://purl.org/dc/elements/1.1/date"/>
        <rdfs:domain rdf:resource="http://www.owl-ontologies.com/Ontology1482491841.owl#LearningOpportunityInstance"/>
        <rdfs:range rdf:resource="http://www.w3.org/2000/01/rdf-schema#Literal"/>
        <rdfs:comment>Definition: A duration of the Learning Opportunity Instance.
Comments: Recommended best practice is to use an encoding scheme, such as the W3CDTF profile of
ISO\-8601.</rdfs:comment>
        <rdfs:label>Duration</rdfs:label>
    </owl:DatatypeProperty>
    


    <!-- http://www.owl-ontologies.com/Ontology1482491841.owl#engagement -->

    <owl:DatatypeProperty rdf:about="http://www.owl-ontologies.com/Ontology1482491841.owl#engagement">
        <rdfs:domain rdf:resource="http://www.owl-ontologies.com/Ontology1482491841.owl#LearningOpportunityInstance"/>
        <rdfs:range rdf:resource="http://www.w3.org/2000/01/rdf-schema#Literal"/>
        <rdfs:comment>Definition: The logistical means by which individuals engage in a Learning Opportunity Instance,
encompassing temporal, modal and spatial patterns of engagement and attendance.
Comments: Examples include overall attendance (full-time, part-time), modes of study (distance, campusbased,
workplace-based, online), and patterns of attendance hours (evenings, daytime,
weekend). Attention is drawn to http://purl.org/dc/elements/1.1/coverage as a similar, though not
equivalent, property.</rdfs:comment>
        <rdfs:label>Engagement</rdfs:label>
    </owl:DatatypeProperty>
    


    <!-- http://www.owl-ontologies.com/Ontology1482491841.owl#languageOfInstruction -->

    <owl:DatatypeProperty rdf:about="http://www.owl-ontologies.com/Ontology1482491841.owl#languageOfInstruction">
        <rdfs:domain rdf:resource="http://www.owl-ontologies.com/Ontology1482491841.owl#LearningOpportunityInstance"/>
        <rdfs:range rdf:resource="http://www.w3.org/2000/01/rdf-schema#Literal"/>
        <rdfs:comment>Definition: A language in which the Learning Opportunity Instance is available to be taught.
Comments: Attention is drawn to ISO\-639.</rdfs:comment>
        <rdfs:label>Language of instruction</rdfs:label>
    </owl:DatatypeProperty>
    


    <!-- http://www.owl-ontologies.com/Ontology1482491841.owl#level -->

    <owl:DatatypeProperty rdf:about="http://www.owl-ontologies.com/Ontology1482491841.owl#level">
        <rdfs:domain rdf:resource="http://www.owl-ontologies.com/Ontology1482491841.owl#LearningOpportunitySpecification"/>
        <rdfs:range rdf:resource="http://www.w3.org/2000/01/rdf-schema#Literal"/>
        <rdfs:comment>Definition: An account of the education level of the Learning Opportunity.
Comments: Level will typically indicate the intended outcome of the Learning Opportunity in terms of
progression; contrast this with the Prerequisite property. Attention is drawn to
http://purl.org/dc/terms/educationLevel as defined in DCMI\-TERMS as a similar, though not
equivalent term.</rdfs:comment>
        <rdfs:label>Level</rdfs:label>
    </owl:DatatypeProperty>
    


    <!-- http://www.owl-ontologies.com/Ontology1482491841.owl#location -->

    <owl:DatatypeProperty rdf:about="http://www.owl-ontologies.com/Ontology1482491841.owl#location">
        <rdfs:domain rdf:resource="http://www.owl-ontologies.com/Ontology1482491841.owl#LearningOpportunityInstance"/>
        <rdfs:domain rdf:resource="http://www.owl-ontologies.com/Ontology1482491841.owl#LearningOpportunityProvider"/>
        <rdfs:range rdf:resource="http://www.w3.org/2000/01/rdf-schema#Resource"/>
        <rdfs:comment>Definition: The spatial location of the Learning Opportunity Provider or Learning Opportunity Instance
Relations.
Comments: Typically an address and/or geographic co-ordinates. Attention is drawn to UPU\-S42,
EN14142\-1 and GEO\-RSS.</rdfs:comment>
        <rdfs:label>Location</rdfs:label>
    </owl:DatatypeProperty>
    


    <!-- http://www.owl-ontologies.com/Ontology1482491841.owl#objective -->

    <owl:DatatypeProperty rdf:about="http://www.owl-ontologies.com/Ontology1482491841.owl#objective">
        <rdfs:domain rdf:resource="http://www.owl-ontologies.com/Ontology1482491841.owl#LearningOpportunityInstance"/>
        <rdfs:range rdf:resource="http://www.w3.org/2000/01/rdf-schema#Resource"/>
        <rdfs:comment>Definition: An aim or learning objective for the Learning Opportunity Instance.
Comments:</rdfs:comment>
        <rdfs:label>Objective</rdfs:label>
    </owl:DatatypeProperty>
    


    <!-- http://www.owl-ontologies.com/Ontology1482491841.owl#places -->

    <owl:DatatypeProperty rdf:about="http://www.owl-ontologies.com/Ontology1482491841.owl#places">
        <rdfs:domain rdf:resource="http://www.owl-ontologies.com/Ontology1482491841.owl#LearningOpportunityInstance"/>
        <rdfs:range rdf:resource="http://www.w3.org/2000/01/rdf-schema#Resource"/>
        <rdfs:comment>Definition: Number of places available for participants in the Learning Opportunity Instance
Comments:</rdfs:comment>
        <rdfs:label>Places</rdfs:label>
    </owl:DatatypeProperty>
    


    <!-- http://www.owl-ontologies.com/Ontology1482491841.owl#prerequisite -->

    <owl:DatatypeProperty rdf:about="http://www.owl-ontologies.com/Ontology1482491841.owl#prerequisite">
        <rdfs:domain rdf:resource="http://www.owl-ontologies.com/Ontology1482491841.owl#LearningOpportunityInstance"/>
        <rdfs:range rdf:resource="http://www.w3.org/2000/01/rdf-schema#Resource"/>
        <rdfs:comment>Definition: A prerequisite or entry requirement for accessing the Learning Opportunity Instance.
Comments:</rdfs:comment>
        <rdfs:label>Prerequisite</rdfs:label>
    </owl:DatatypeProperty>
    


    <!-- http://www.owl-ontologies.com/Ontology1482491841.owl#qualification -->

    <owl:DatatypeProperty rdf:about="http://www.owl-ontologies.com/Ontology1482491841.owl#qualification">
        <rdfs:domain rdf:resource="http://www.owl-ontologies.com/Ontology1482491841.owl#LearningOpportunitySpecification"/>
        <rdfs:range rdf:resource="http://www.w3.org/2000/01/rdf-schema#Resource"/>
        <rdfs:comment>Definition: A qualification that can be obtained from completion of a Learning Opportunity.
Comments:</rdfs:comment>
        <rdfs:label>Qualification</rdfs:label>
    </owl:DatatypeProperty>
    


    <!-- http://www.owl-ontologies.com/Ontology1482491841.owl#start -->

    <owl:DatatypeProperty rdf:about="http://www.owl-ontologies.com/Ontology1482491841.owl#start">
        <rdfs:subPropertyOf rdf:resource="http://purl.org/dc/elements/1.1/date"/>
        <rdfs:domain rdf:resource="http://www.owl-ontologies.com/Ontology1482491841.owl#LearningOpportunityInstance"/>
        <rdfs:range rdf:resource="http://www.w3.org/2000/01/rdf-schema#Literal"/>
        <rdfs:comment>Definition: A date from which the Learning Opportunity Instance commences.
Comments: Recommended best practice is to use an encoding scheme, such as the W3CDTF profile of
ISO\-8601.</rdfs:comment>
        <rdfs:label>Start</rdfs:label>
    </owl:DatatypeProperty>
    


    <!-- http://www.owl-ontologies.com/Ontology1482491841.owl#url -->

    <owl:DatatypeProperty rdf:about="http://www.owl-ontologies.com/Ontology1482491841.owl#url">
        <rdfs:domain rdf:resource="http://www.owl-ontologies.com/Ontology1482491841.owl#LearningOpportunityObject"/>
        <rdfs:range rdf:resource="http://www.w3.org/2000/01/rdf-schema#Literal"/>
        <rdfs:comment>Definition: A link to a web resource that provides an alternate representation of the resource. The content
should conform to a URI IETF\-RFC2396.
Comments: Typically the web page of the provider or course.</rdfs:comment>
        <rdfs:label>Url</rdfs:label>
    </owl:DatatypeProperty>
    


    <!-- 
    ///////////////////////////////////////////////////////////////////////////////////////
    //
    // Classes
    //
    ///////////////////////////////////////////////////////////////////////////////////////
     -->

    


    <!-- http://www.owl-ontologies.com/Ontology1482491841.owl#LearningOpportunityInstance -->

    <owl:Class rdf:about="http://www.owl-ontologies.com/Ontology1482491841.owl#LearningOpportunityInstance">
        <rdfs:subClassOf rdf:resource="http://www.owl-ontologies.com/Ontology1482491841.owl#LearningOpportunityObject"/>
    </owl:Class>
    


    <!-- http://www.owl-ontologies.com/Ontology1482491841.owl#LearningOpportunityObject -->

    <owl:Class rdf:about="http://www.owl-ontologies.com/Ontology1482491841.owl#LearningOpportunityObject">
        <rdfs:comment>Definition: An abstract resource used within the context of learning opportunities.
Comments:</rdfs:comment>
        <rdfs:label>Learning Opportunity Object</rdfs:label>
    </owl:Class>
    


    <!-- http://www.owl-ontologies.com/Ontology1482491841.owl#LearningOpportunityProvider -->

    <owl:Class rdf:about="http://www.owl-ontologies.com/Ontology1482491841.owl#LearningOpportunityProvider">
        <rdfs:subClassOf rdf:resource="http://www.owl-ontologies.com/Ontology1482491841.owl#LearningOpportunityObject"/>
        <rdfs:comment>Definition: An agent (person or organisation) that provides learning opportunities.
Comments:</rdfs:comment>
        <rdfs:label>Learning Opportunity Provider</rdfs:label>
    </owl:Class>
    


    <!-- http://www.owl-ontologies.com/Ontology1482491841.owl#LearningOpportunitySpecification -->

    <owl:Class rdf:about="http://www.owl-ontologies.com/Ontology1482491841.owl#LearningOpportunitySpecification">
        <rdfs:subClassOf rdf:resource="http://www.owl-ontologies.com/Ontology1482491841.owl#LearningOpportunityObject"/>
        <rdfs:comment>Definition: An abstract description of a learning opportunity, consisting of information that will be
consistent across multiple instances of the learning opportunity.
Comments:</rdfs:comment>
        <rdfs:label>Learning Opportunity Specification</rdfs:label>
    </owl:Class>
    


    <!-- 
    ///////////////////////////////////////////////////////////////////////////////////////
    //
    // Annotations
    //
    ///////////////////////////////////////////////////////////////////////////////////////
     -->

    <rdf:Description rdf:about="http://purl.org/dc/elements/1.1/">
        <terms:publisher rdf:resource="http://purl.org/dc/aboutdcmi#DCMI"/>
        <terms:title xml:lang="en">Dublin Core Metadata Element Set, Version 1.1</terms:title>
        <terms:modified rdf:datatype="http://www.w3.org/2001/XMLSchema#date">2012-06-14</terms:modified>
    </rdf:Description>
    <rdf:Description rdf:about="http://purl.org/dc/elements/1.1/contributor">
        <rdfs:label xml:lang="en">Contributor</rdfs:label>
        <terms:hasVersion rdf:resource="http://dublincore.org/usage/terms/history/#contributor-006"/>
        <skos:note xml:lang="en">A second property with the same name as this property has been declared in the dcterms: namespace (http://purl.org/dc/terms/).  See the Introduction to the document &quot;DCMI Metadata Terms&quot; (http://dublincore.org/documents/dcmi-terms/) for an explanation.</skos:note>
        <rdfs:comment xml:lang="en">An entity responsible for making contributions to the resource.</rdfs:comment>
        <terms:description xml:lang="en">Examples of a Contributor include a person, an organization, or a service. Typically, the name of a Contributor should be used to indicate the entity.</terms:description>
        <terms:modified rdf:datatype="http://www.w3.org/2001/XMLSchema#date">2008-01-14</terms:modified>
        <terms:issued rdf:datatype="http://www.w3.org/2001/XMLSchema#date">1999-07-02</terms:issued>
        <rdfs:isDefinedBy rdf:resource="http://purl.org/dc/elements/1.1/"/>
    </rdf:Description>
    <rdf:Description rdf:about="http://purl.org/dc/elements/1.1/coverage">
        <terms:hasVersion rdf:resource="http://dublincore.org/usage/terms/history/#coverage-006"/>
        <rdfs:isDefinedBy rdf:resource="http://purl.org/dc/elements/1.1/"/>
        <terms:modified rdf:datatype="http://www.w3.org/2001/XMLSchema#date">2008-01-14</terms:modified>
        <skos:note xml:lang="en">A second property with the same name as this property has been declared in the dcterms: namespace (http://purl.org/dc/terms/).  See the Introduction to the document &quot;DCMI Metadata Terms&quot; (http://dublincore.org/documents/dcmi-terms/) for an explanation.</skos:note>
        <rdfs:comment xml:lang="en">The spatial or temporal topic of the resource, the spatial applicability of the resource, or the jurisdiction under which the resource is relevant.</rdfs:comment>
        <terms:description xml:lang="en">Spatial topic and spatial applicability may be a named place or a location specified by its geographic coordinates. Temporal topic may be a named period, date, or date range. A jurisdiction may be a named administrative entity or a geographic place to which the resource applies. Recommended best practice is to use a controlled vocabulary such as the Thesaurus of Geographic Names [TGN]. Where appropriate, named places or time periods can be used in preference to numeric identifiers such as sets of coordinates or date ranges.</terms:description>
        <terms:issued rdf:datatype="http://www.w3.org/2001/XMLSchema#date">1999-07-02</terms:issued>
        <rdfs:label xml:lang="en">Coverage</rdfs:label>
    </rdf:Description>
    <rdf:Description rdf:about="http://purl.org/dc/elements/1.1/creator">
        <terms:modified rdf:datatype="http://www.w3.org/2001/XMLSchema#date">2008-01-14</terms:modified>
        <rdfs:label xml:lang="en">Creator</rdfs:label>
        <rdfs:comment xml:lang="en">An entity primarily responsible for making the resource.</rdfs:comment>
        <rdfs:isDefinedBy rdf:resource="http://purl.org/dc/elements/1.1/"/>
        <terms:description xml:lang="en">Examples of a Creator include a person, an organization, or a service. Typically, the name of a Creator should be used to indicate the entity.</terms:description>
        <terms:hasVersion rdf:resource="http://dublincore.org/usage/terms/history/#creator-006"/>
        <skos:note xml:lang="en">A second property with the same name as this property has been declared in the dcterms: namespace (http://purl.org/dc/terms/).  See the Introduction to the document &quot;DCMI Metadata Terms&quot; (http://dublincore.org/documents/dcmi-terms/) for an explanation.</skos:note>
        <terms:issued rdf:datatype="http://www.w3.org/2001/XMLSchema#date">1999-07-02</terms:issued>
    </rdf:Description>
    <rdf:Description rdf:about="http://purl.org/dc/elements/1.1/description">
        <terms:description xml:lang="en">Description may include but is not limited to: an abstract, a table of contents, a graphical representation, or a free-text account of the resource.</terms:description>
        <rdfs:isDefinedBy rdf:resource="http://purl.org/dc/elements/1.1/"/>
        <terms:issued rdf:datatype="http://www.w3.org/2001/XMLSchema#date">1999-07-02</terms:issued>
        <skos:note xml:lang="en">A second property with the same name as this property has been declared in the dcterms: namespace (http://purl.org/dc/terms/).  See the Introduction to the document &quot;DCMI Metadata Terms&quot; (http://dublincore.org/documents/dcmi-terms/) for an explanation.</skos:note>
        <rdfs:comment xml:lang="en">An account of the resource.</rdfs:comment>
        <terms:modified rdf:datatype="http://www.w3.org/2001/XMLSchema#date">2008-01-14</terms:modified>
        <rdfs:label xml:lang="en">Description</rdfs:label>
        <terms:hasVersion rdf:resource="http://dublincore.org/usage/terms/history/#description-006"/>
    </rdf:Description>
    <rdf:Description rdf:about="http://purl.org/dc/elements/1.1/format">
        <skos:note xml:lang="en">A second property with the same name as this property has been declared in the dcterms: namespace (http://purl.org/dc/terms/).  See the Introduction to the document &quot;DCMI Metadata Terms&quot; (http://dublincore.org/documents/dcmi-terms/) for an explanation.</skos:note>
        <terms:issued rdf:datatype="http://www.w3.org/2001/XMLSchema#date">1999-07-02</terms:issued>
        <terms:modified rdf:datatype="http://www.w3.org/2001/XMLSchema#date">2008-01-14</terms:modified>
        <rdfs:label xml:lang="en">Format</rdfs:label>
        <rdfs:comment xml:lang="en">The file format, physical medium, or dimensions of the resource.</rdfs:comment>
        <terms:hasVersion rdf:resource="http://dublincore.org/usage/terms/history/#format-007"/>
        <rdfs:isDefinedBy rdf:resource="http://purl.org/dc/elements/1.1/"/>
        <terms:description xml:lang="en">Examples of dimensions include size and duration. Recommended best practice is to use a controlled vocabulary such as the list of Internet Media Types [MIME].</terms:description>
    </rdf:Description>
    <rdf:Description rdf:about="http://purl.org/dc/elements/1.1/identifier">
        <terms:hasVersion rdf:resource="http://dublincore.org/usage/terms/history/#identifier-006"/>
        <rdfs:isDefinedBy rdf:resource="http://purl.org/dc/elements/1.1/"/>
        <terms:description xml:lang="en">Recommended best practice is to identify the resource by means of a string conforming to a formal identification system. </terms:description>
        <rdfs:comment xml:lang="en">An unambiguous reference to the resource within a given context.</rdfs:comment>
        <terms:issued rdf:datatype="http://www.w3.org/2001/XMLSchema#date">1999-07-02</terms:issued>
        <terms:modified rdf:datatype="http://www.w3.org/2001/XMLSchema#date">2008-01-14</terms:modified>
        <rdfs:label xml:lang="en">Identifier</rdfs:label>
        <skos:note xml:lang="en">A second property with the same name as this property has been declared in the dcterms: namespace (http://purl.org/dc/terms/).  See the Introduction to the document &quot;DCMI Metadata Terms&quot; (http://dublincore.org/documents/dcmi-terms/) for an explanation.</skos:note>
    </rdf:Description>
    <rdf:Description rdf:about="http://purl.org/dc/elements/1.1/language">
        <terms:modified rdf:datatype="http://www.w3.org/2001/XMLSchema#date">2008-01-14</terms:modified>
        <terms:issued rdf:datatype="http://www.w3.org/2001/XMLSchema#date">1999-07-02</terms:issued>
        <skos:note xml:lang="en">A second property with the same name as this property has been declared in the dcterms: namespace (http://purl.org/dc/terms/).  See the Introduction to the document &quot;DCMI Metadata Terms&quot; (http://dublincore.org/documents/dcmi-terms/) for an explanation.</skos:note>
        <terms:hasVersion rdf:resource="http://dublincore.org/usage/terms/history/#language-007"/>
        <rdfs:label xml:lang="en">Language</rdfs:label>
        <terms:description xml:lang="en">Recommended best practice is to use a controlled vocabulary such as RFC 4646 [RFC4646].</terms:description>
        <rdfs:isDefinedBy rdf:resource="http://purl.org/dc/elements/1.1/"/>
        <rdfs:comment xml:lang="en">A language of the resource.</rdfs:comment>
        <rdfs:seeAlso rdf:resource="http://www.ietf.org/rfc/rfc4646.txt"/>
    </rdf:Description>
    <rdf:Description rdf:about="http://purl.org/dc/elements/1.1/publisher">
        <terms:hasVersion rdf:resource="http://dublincore.org/usage/terms/history/#publisher-006"/>
        <skos:note xml:lang="en">A second property with the same name as this property has been declared in the dcterms: namespace (http://purl.org/dc/terms/).  See the Introduction to the document &quot;DCMI Metadata Terms&quot; (http://dublincore.org/documents/dcmi-terms/) for an explanation.</skos:note>
        <terms:issued rdf:datatype="http://www.w3.org/2001/XMLSchema#date">1999-07-02</terms:issued>
        <terms:modified rdf:datatype="http://www.w3.org/2001/XMLSchema#date">2008-01-14</terms:modified>
        <rdfs:label xml:lang="en">Publisher</rdfs:label>
        <rdfs:isDefinedBy rdf:resource="http://purl.org/dc/elements/1.1/"/>
        <terms:description xml:lang="en">Examples of a Publisher include a person, an organization, or a service. Typically, the name of a Publisher should be used to indicate the entity.</terms:description>
        <rdfs:comment xml:lang="en">An entity responsible for making the resource available.</rdfs:comment>
    </rdf:Description>
    <rdf:Description rdf:about="http://purl.org/dc/elements/1.1/relation">
        <terms:hasVersion rdf:resource="http://dublincore.org/usage/terms/history/#relation-006"/>
        <terms:description xml:lang="en">Recommended best practice is to identify the related resource by means of a string conforming to a formal identification system. </terms:description>
        <rdfs:label xml:lang="en">Relation</rdfs:label>
        <terms:modified rdf:datatype="http://www.w3.org/2001/XMLSchema#date">2008-01-14</terms:modified>
        <terms:issued rdf:datatype="http://www.w3.org/2001/XMLSchema#date">1999-07-02</terms:issued>
        <skos:note xml:lang="en">A second property with the same name as this property has been declared in the dcterms: namespace (http://purl.org/dc/terms/).  See the Introduction to the document &quot;DCMI Metadata Terms&quot; (http://dublincore.org/documents/dcmi-terms/) for an explanation.</skos:note>
        <rdfs:comment xml:lang="en">A related resource.</rdfs:comment>
        <rdfs:isDefinedBy rdf:resource="http://purl.org/dc/elements/1.1/"/>
    </rdf:Description>
    <rdf:Description rdf:about="http://purl.org/dc/elements/1.1/rights">
        <terms:hasVersion rdf:resource="http://dublincore.org/usage/terms/history/#rights-006"/>
        <rdfs:isDefinedBy rdf:resource="http://purl.org/dc/elements/1.1/"/>
        <skos:note xml:lang="en">A second property with the same name as this property has been declared in the dcterms: namespace (http://purl.org/dc/terms/).  See the Introduction to the document &quot;DCMI Metadata Terms&quot; (http://dublincore.org/documents/dcmi-terms/) for an explanation.</skos:note>
        <terms:issued rdf:datatype="http://www.w3.org/2001/XMLSchema#date">1999-07-02</terms:issued>
        <terms:description xml:lang="en">Typically, rights information includes a statement about various property rights associated with the resource, including intellectual property rights.</terms:description>
        <rdfs:label xml:lang="en">Rights</rdfs:label>
        <terms:modified rdf:datatype="http://www.w3.org/2001/XMLSchema#date">2008-01-14</terms:modified>
        <rdfs:comment xml:lang="en">Information about rights held in and over the resource.</rdfs:comment>
    </rdf:Description>
    <rdf:Description rdf:about="http://purl.org/dc/elements/1.1/source">
        <terms:hasVersion rdf:resource="http://dublincore.org/usage/terms/history/#source-006"/>
        <skos:note xml:lang="en">A second property with the same name as this property has been declared in the dcterms: namespace (http://purl.org/dc/terms/).  See the Introduction to the document &quot;DCMI Metadata Terms&quot; (http://dublincore.org/documents/dcmi-terms/) for an explanation.</skos:note>
        <rdfs:isDefinedBy rdf:resource="http://purl.org/dc/elements/1.1/"/>
        <rdfs:comment xml:lang="en">A related resource from which the described resource is derived.</rdfs:comment>
        <terms:modified rdf:datatype="http://www.w3.org/2001/XMLSchema#date">2008-01-14</terms:modified>
        <terms:description xml:lang="en">The described resource may be derived from the related resource in whole or in part. Recommended best practice is to identify the related resource by means of a string conforming to a formal identification system.</terms:description>
        <terms:issued rdf:datatype="http://www.w3.org/2001/XMLSchema#date">1999-07-02</terms:issued>
        <rdfs:label xml:lang="en">Source</rdfs:label>
    </rdf:Description>
    <rdf:Description rdf:about="http://purl.org/dc/elements/1.1/subject">
        <terms:description xml:lang="en">Typically, the subject will be represented using keywords, key phrases, or classification codes. Recommended best practice is to use a controlled vocabulary.</terms:description>
        <skos:note xml:lang="en">A second property with the same name as this property has been declared in the dcterms: namespace (http://purl.org/dc/terms/).  See the Introduction to the document &quot;DCMI Metadata Terms&quot; (http://dublincore.org/documents/dcmi-terms/) for an explanation.</skos:note>
        <terms:issued rdf:datatype="http://www.w3.org/2001/XMLSchema#date">1999-07-02</terms:issued>
        <rdfs:label xml:lang="en">Subject</rdfs:label>
        <rdfs:comment xml:lang="en">The topic of the resource.</rdfs:comment>
        <rdfs:isDefinedBy rdf:resource="http://purl.org/dc/elements/1.1/"/>
        <terms:modified rdf:datatype="http://www.w3.org/2001/XMLSchema#date">2012-06-14</terms:modified>
        <terms:hasVersion rdf:resource="http://dublincore.org/usage/terms/history/#subject-007"/>
    </rdf:Description>
    <rdf:Description rdf:about="http://purl.org/dc/elements/1.1/title">
        <rdfs:comment xml:lang="en">A name given to the resource.</rdfs:comment>
        <terms:modified rdf:datatype="http://www.w3.org/2001/XMLSchema#date">2008-01-14</terms:modified>
        <skos:note xml:lang="en">A second property with the same name as this property has been declared in the dcterms: namespace (http://purl.org/dc/terms/).  See the Introduction to the document &quot;DCMI Metadata Terms&quot; (http://dublincore.org/documents/dcmi-terms/) for an explanation.</skos:note>
        <rdfs:label xml:lang="en">Title</rdfs:label>
        <terms:issued rdf:datatype="http://www.w3.org/2001/XMLSchema#date">1999-07-02</terms:issued>
        <terms:hasVersion rdf:resource="http://dublincore.org/usage/terms/history/#title-006"/>
        <rdfs:isDefinedBy rdf:resource="http://purl.org/dc/elements/1.1/"/>
    </rdf:Description>
    <rdf:Description rdf:about="http://purl.org/dc/elements/1.1/type">
        <terms:hasVersion rdf:resource="http://dublincore.org/usage/terms/history/#type-006"/>
        <rdfs:comment xml:lang="en">The nature or genre of the resource.</rdfs:comment>
        <rdfs:label xml:lang="en">Type</rdfs:label>
        <rdfs:isDefinedBy rdf:resource="http://purl.org/dc/elements/1.1/"/>
        <terms:description xml:lang="en">Recommended best practice is to use a controlled vocabulary such as the DCMI Type Vocabulary [DCMITYPE]. To describe the file format, physical medium, or dimensions of the resource, use the Format element.</terms:description>
        <terms:issued rdf:datatype="http://www.w3.org/2001/XMLSchema#date">1999-07-02</terms:issued>
        <skos:note xml:lang="en">A second property with the same name as this property has been declared in the dcterms: namespace (http://purl.org/dc/terms/).  See the Introduction to the document &quot;DCMI Metadata Terms&quot; (http://dublincore.org/documents/dcmi-terms/) for an explanation.</skos:note>
        <terms:modified rdf:datatype="http://www.w3.org/2001/XMLSchema#date">2008-01-14</terms:modified>
    </rdf:Description>
    <rdf:Description rdf:about="http://www.owl-ontologies.com/Ontology1482491841.owl#LearningOpportunityInstance">
        <rdfs:comment>Learning Opportunity Instance</rdfs:comment>
        <rdfs:comment>Definition: A single occurrence of a learning opportunity. Unlike a Learning Opportunity Specification, a
Learning Opportunity Instance is not abstract, may be bound to particular dates or locations, and
may be applied for or participated in by learners.
Comments:</rdfs:comment>
        <rdfs:label>Learning Opportunity Instance</rdfs:label>
    </rdf:Description>
    


    <!-- 
    ///////////////////////////////////////////////////////////////////////////////////////
    //
    // General axioms
    //
    ///////////////////////////////////////////////////////////////////////////////////////
     -->

    <rdf:Description>
        <rdf:type rdf:resource="http://www.w3.org/2002/07/owl#AllDisjointClasses"/>
        <owl:members rdf:parseType="Collection">
            <rdf:Description rdf:about="http://www.owl-ontologies.com/Ontology1482491841.owl#LearningOpportunityInstance"/>
            <rdf:Description rdf:about="http://www.owl-ontologies.com/Ontology1482491841.owl#LearningOpportunityProvider"/>
            <rdf:Description rdf:about="http://www.owl-ontologies.com/Ontology1482491841.owl#LearningOpportunitySpecification"/>
        </owl:members>
    </rdf:Description>
</rdf:RDF>



<!-- Generated by the OWL API (version 4.2.6.20160910-2108) https://github.com/owlcs/owlapi -->

