<?xml version="1.0"?>
<rdf:RDF xmlns="http://www.semanticweb.org/nina/ontologies/2016/11/erasmus#"
     xml:base="http://www.semanticweb.org/nina/ontologies/2016/11/erasmus"
     xmlns:rdf="http://www.w3.org/1999/02/22-rdf-syntax-ns#"
     xmlns:terms="http://purl.org/dc/terms/"
     xmlns:owl="http://www.w3.org/2002/07/owl#"
     xmlns:erasmus="http://www.semanticweb.org/nina/ontologies/2016/11/erasmus#"
     xmlns:xml="http://www.w3.org/XML/1998/namespace"
     xmlns:xsd="http://www.w3.org/2001/XMLSchema#"
     xmlns:skos="http://www.w3.org/2004/02/skos/core#"
     xmlns:rdfs="http://www.w3.org/2000/01/rdf-schema#"
     xmlns:dc="http://purl.org/dc/elements/1.1">
    <owl:Ontology rdf:about="http://www.semanticweb.org/nina/ontologies/2016/11/erasmus">
        <owl:imports rdf:resource="http://purl.org/dc/elements/1.1"/>
    </owl:Ontology>
    


    <!-- 
    ///////////////////////////////////////////////////////////////////////////////////////
    //
    // Annotation properties
    //
    ///////////////////////////////////////////////////////////////////////////////////////
     -->

    


    <!-- http://www.semanticweb.org/nina/ontologies/2016/11/erasmus#hasCourseUnitInformation -->

    <owl:AnnotationProperty rdf:about="http://www.semanticweb.org/nina/ontologies/2016/11/erasmus#hasCourseUnitInformation">
        <rdfs:subPropertyOf rdf:resource="http://purl.org/dc/terms/description"/>
    </owl:AnnotationProperty>
    


    <!-- http://www.semanticweb.org/nina/ontologies/2016/11/erasmus#hasDegreeProgrammeInformation -->

    <owl:AnnotationProperty rdf:about="http://www.semanticweb.org/nina/ontologies/2016/11/erasmus#hasDegreeProgrammeInformation">
        <rdfs:subPropertyOf rdf:resource="http://purl.org/dc/terms/description"/>
    </owl:AnnotationProperty>
    


    <!-- http://www.semanticweb.org/nina/ontologies/2016/11/erasmus#hasGeneralInformationForStudents -->

    <owl:AnnotationProperty rdf:about="http://www.semanticweb.org/nina/ontologies/2016/11/erasmus#hasGeneralInformationForStudents">
        <rdfs:subPropertyOf rdf:resource="http://purl.org/dc/terms/description"/>
    </owl:AnnotationProperty>
    


    <!-- http://www.semanticweb.org/nina/ontologies/2016/11/erasmus#hasInstitutionDescription -->

    <owl:AnnotationProperty rdf:about="http://www.semanticweb.org/nina/ontologies/2016/11/erasmus#hasInstitutionDescription">
        <rdfs:subPropertyOf rdf:resource="http://purl.org/dc/terms/description"/>
    </owl:AnnotationProperty>
    


    <!-- 
    ///////////////////////////////////////////////////////////////////////////////////////
    //
    // Object Properties
    //
    ///////////////////////////////////////////////////////////////////////////////////////
     -->

    


    <!-- http://www.semanticweb.org/nina/ontologies/2016/11/erasmus#hasPart -->

    <owl:ObjectProperty rdf:about="http://www.semanticweb.org/nina/ontologies/2016/11/erasmus#hasPart">
        <rdfs:subPropertyOf rdf:resource="http://www.w3.org/2002/07/owl#topObjectProperty"/>
        <rdfs:comment>A relation to a Learning Opportunity Object that is logically included in the Learning Opportunity 
Object.</rdfs:comment>
        <rdfs:label>Has Part</rdfs:label>
    </owl:ObjectProperty>
    


    <!-- http://www.semanticweb.org/nina/ontologies/2016/11/erasmus#offeredAt -->

    <owl:ObjectProperty rdf:about="http://www.semanticweb.org/nina/ontologies/2016/11/erasmus#offeredAt">
        <rdfs:domain rdf:resource="http://www.semanticweb.org/nina/ontologies/2016/11/erasmus#LearningOpportunityInstance"/>
        <rdfs:range rdf:resource="http://www.semanticweb.org/nina/ontologies/2016/11/erasmus#LearningOpportunityProvider"/>
        <rdfs:comment>This can be used to represent franchises or other circumstances when the provider that offers
the instance is different to the provider that defines the specification. Content should be a URI
conforming to IETF\-RFC2396.</rdfs:comment>
        <rdfs:label>Offered At</rdfs:label>
    </owl:ObjectProperty>
    


    <!-- http://www.semanticweb.org/nina/ontologies/2016/11/erasmus#offers -->

    <owl:ObjectProperty rdf:about="http://www.semanticweb.org/nina/ontologies/2016/11/erasmus#offers">
        <rdfs:subPropertyOf rdf:resource="http://www.w3.org/2002/07/owl#topObjectProperty"/>
        <rdfs:domain rdf:resource="http://www.semanticweb.org/nina/ontologies/2016/11/erasmus#LearningOpportunityProvider"/>
        <rdfs:range rdf:resource="http://www.semanticweb.org/nina/ontologies/2016/11/erasmus#LearningOpportunitySpecification"/>
        <rdfs:comment>A relation to a Learning Opportunity Specification offered by the Learning Opportunity Provider.</rdfs:comment>
        <rdfs:label>Offers</rdfs:label>
    </owl:ObjectProperty>
    


    <!-- http://www.semanticweb.org/nina/ontologies/2016/11/erasmus#specifies -->

    <owl:ObjectProperty rdf:about="http://www.semanticweb.org/nina/ontologies/2016/11/erasmus#specifies">
        <rdfs:subPropertyOf rdf:resource="http://www.w3.org/2002/07/owl#topObjectProperty"/>
        <rdfs:domain rdf:resource="http://www.semanticweb.org/nina/ontologies/2016/11/erasmus#LearningOpportunitySpecification"/>
        <rdfs:range rdf:resource="http://www.semanticweb.org/nina/ontologies/2016/11/erasmus#LearningOpportunityInstance"/>
        <rdfs:comment>A relation to a Learning Opportunity Instance that is an instance specified by the Learning
Opportunity Specification.</rdfs:comment>
        <rdfs:label>Specifies</rdfs:label>
    </owl:ObjectProperty>
    


    <!-- 
    ///////////////////////////////////////////////////////////////////////////////////////
    //
    // Data properties
    //
    ///////////////////////////////////////////////////////////////////////////////////////
     -->

    


    <!-- http://www.semanticweb.org/nina/ontologies/2016/11/erasmus#assessment -->

    <owl:DatatypeProperty rdf:about="http://www.semanticweb.org/nina/ontologies/2016/11/erasmus#assessment">
        <rdfs:subPropertyOf rdf:resource="http://www.w3.org/2002/07/owl#topDataProperty"/>
        <rdfs:domain rdf:resource="http://www.semanticweb.org/nina/ontologies/2016/11/erasmus#LearningOpportunityInstance"/>
        <rdfs:range rdf:resource="http://www.w3.org/2001/XMLSchema#string"/>
        <rdfs:comment>Definition: assessment strategy: a description of the broad approach to assessment used in the learning
opportunity.
Comments: Examples include types of assessments and evaluations of learning and competency
development such as exams, mostly by coursework etc.</rdfs:comment>
        <rdfs:label>Assessment</rdfs:label>
    </owl:DatatypeProperty>
    


    <!-- http://www.semanticweb.org/nina/ontologies/2016/11/erasmus#cost -->

    <owl:DatatypeProperty rdf:about="http://www.semanticweb.org/nina/ontologies/2016/11/erasmus#cost">
        <rdfs:subPropertyOf rdf:resource="http://www.w3.org/2002/07/owl#topDataProperty"/>
        <rdfs:domain rdf:resource="http://www.semanticweb.org/nina/ontologies/2016/11/erasmus#LearningOpportunityInstance"/>
        <rdfs:range rdf:resource="http://www.w3.org/2000/01/rdf-schema#Literal"/>
        <rdfs:comment>A cost associated with obtaining access to the Learning Opportunity Instance.</rdfs:comment>
        <rdfs:label>Cost</rdfs:label>
    </owl:DatatypeProperty>
    


    <!-- http://www.semanticweb.org/nina/ontologies/2016/11/erasmus#credit -->

    <owl:DatatypeProperty rdf:about="http://www.semanticweb.org/nina/ontologies/2016/11/erasmus#credit">
        <rdfs:subPropertyOf rdf:resource="http://www.w3.org/2002/07/owl#topDataProperty"/>
        <rdfs:domain rdf:resource="http://www.semanticweb.org/nina/ontologies/2016/11/erasmus#LearningOpportunitySpecification"/>
        <rdfs:range rdf:resource="http://www.w3.org/2001/XMLSchema#string"/>
        <rdfs:comment>An account of the credits that can be obtained from completion of a Learning Opportunity.</rdfs:comment>
        <rdfs:label>Credit</rdfs:label>
    </owl:DatatypeProperty>
    


    <!-- http://www.semanticweb.org/nina/ontologies/2016/11/erasmus#duration -->

    <owl:DatatypeProperty rdf:about="http://www.semanticweb.org/nina/ontologies/2016/11/erasmus#duration">
        <rdfs:subPropertyOf rdf:resource="http://www.w3.org/2002/07/owl#topDataProperty"/>
        <rdfs:domain rdf:resource="http://www.semanticweb.org/nina/ontologies/2016/11/erasmus#LearningOpportunityInstance"/>
        <rdfs:range rdf:resource="http://www.w3.org/2000/01/rdf-schema#Literal"/>
        <rdfs:comment>A duration of the Learning Opportunity Instance.</rdfs:comment>
        <rdfs:label>Duration</rdfs:label>
    </owl:DatatypeProperty>
    


    <!-- http://www.semanticweb.org/nina/ontologies/2016/11/erasmus#engagement -->

    <owl:DatatypeProperty rdf:about="http://www.semanticweb.org/nina/ontologies/2016/11/erasmus#engagement">
        <rdfs:subPropertyOf rdf:resource="http://www.w3.org/2002/07/owl#topDataProperty"/>
        <rdfs:domain rdf:resource="http://www.semanticweb.org/nina/ontologies/2016/11/erasmus#LearningOpportunityInstance"/>
        <rdfs:range rdf:resource="http://www.w3.org/2000/01/rdf-schema#Literal"/>
        <rdfs:comment>The logistical means by which individuals engage in a Learning Opportunity Instance,
encompassing temporal, modal and spatial patterns of engagement and attendance.
 Examples include overall attendance (full-time, part-time), modes of study (distance, campusbased,
workplace-based, online), and patterns of attendance hours (evenings, daytime,
weekend). Attention is drawn to http://purl.org/dc/elements/1.1/coverage as a similar, though not
equivalent, property.</rdfs:comment>
        <rdfs:label>Engagement</rdfs:label>
    </owl:DatatypeProperty>
    


    <!-- http://www.semanticweb.org/nina/ontologies/2016/11/erasmus#languageOfInstruction -->

    <owl:DatatypeProperty rdf:about="http://www.semanticweb.org/nina/ontologies/2016/11/erasmus#languageOfInstruction">
        <rdfs:subPropertyOf rdf:resource="http://www.w3.org/2002/07/owl#topDataProperty"/>
        <rdfs:domain rdf:resource="http://www.semanticweb.org/nina/ontologies/2016/11/erasmus#LearningOpportunityInstance"/>
        <rdfs:range rdf:resource="http://www.w3.org/2000/01/rdf-schema#Literal"/>
        <rdfs:comment>A language in which the Learning Opportunity Instance is available to be taught.</rdfs:comment>
        <rdfs:label>Language Of Instruction</rdfs:label>
    </owl:DatatypeProperty>
    


    <!-- http://www.semanticweb.org/nina/ontologies/2016/11/erasmus#level -->

    <owl:DatatypeProperty rdf:about="http://www.semanticweb.org/nina/ontologies/2016/11/erasmus#level">
        <rdfs:subPropertyOf rdf:resource="http://www.w3.org/2002/07/owl#topDataProperty"/>
        <rdfs:domain rdf:resource="http://www.semanticweb.org/nina/ontologies/2016/11/erasmus#LearningOpportunitySpecification"/>
        <rdfs:range rdf:resource="http://www.w3.org/2000/01/rdf-schema#Literal"/>
        <rdfs:comment>Level will typically indicate the intended outcome of the Learning Opportunity in terms of
progression; contrast this with the Prerequisite property. Attention is drawn to
http://purl.org/dc/terms/educationLevel as defined in DCMI\-TERMS as a similar, though not
equivalent term.</rdfs:comment>
        <rdfs:label>Level</rdfs:label>
    </owl:DatatypeProperty>
    


    <!-- http://www.semanticweb.org/nina/ontologies/2016/11/erasmus#location -->

    <owl:DatatypeProperty rdf:about="http://www.semanticweb.org/nina/ontologies/2016/11/erasmus#location">
        <rdfs:domain rdf:resource="http://www.semanticweb.org/nina/ontologies/2016/11/erasmus#LearningOpportunityInstance"/>
        <rdfs:domain rdf:resource="http://www.semanticweb.org/nina/ontologies/2016/11/erasmus#LearningOpportunityProvider"/>
        <rdfs:range rdf:resource="http://www.w3.org/2001/XMLSchema#string"/>
        <rdfs:comment>Typically an address and/or geographic co-ordinates. Attention is drawn to UPU\-S42,
EN14142\-1 and GEO\-RSS.</rdfs:comment>
        <rdfs:label>Location</rdfs:label>
    </owl:DatatypeProperty>
    


    <!-- http://www.semanticweb.org/nina/ontologies/2016/11/erasmus#objective -->

    <owl:DatatypeProperty rdf:about="http://www.semanticweb.org/nina/ontologies/2016/11/erasmus#objective">
        <rdfs:subPropertyOf rdf:resource="http://www.w3.org/2002/07/owl#topDataProperty"/>
        <rdfs:domain rdf:resource="http://www.semanticweb.org/nina/ontologies/2016/11/erasmus#LearningOpportunityInstance"/>
        <rdfs:range rdf:resource="http://www.w3.org/2001/XMLSchema#string"/>
        <rdfs:comment>An aim or learning objective for the Learning Opportunity Instance.</rdfs:comment>
        <rdfs:label>Objective</rdfs:label>
    </owl:DatatypeProperty>
    


    <!-- http://www.semanticweb.org/nina/ontologies/2016/11/erasmus#places -->

    <owl:DatatypeProperty rdf:about="http://www.semanticweb.org/nina/ontologies/2016/11/erasmus#places">
        <rdfs:subPropertyOf rdf:resource="http://www.w3.org/2002/07/owl#topDataProperty"/>
        <rdfs:domain rdf:resource="http://www.semanticweb.org/nina/ontologies/2016/11/erasmus#LearningOpportunityInstance"/>
        <rdfs:range rdf:resource="http://www.w3.org/2001/XMLSchema#string"/>
        <rdfs:comment>Number of places available for participants in the Learning Opportunity Instance</rdfs:comment>
        <rdfs:label>Places</rdfs:label>
    </owl:DatatypeProperty>
    


    <!-- http://www.semanticweb.org/nina/ontologies/2016/11/erasmus#prerequisite -->

    <owl:DatatypeProperty rdf:about="http://www.semanticweb.org/nina/ontologies/2016/11/erasmus#prerequisite">
        <rdfs:subPropertyOf rdf:resource="http://www.w3.org/2002/07/owl#topDataProperty"/>
        <rdfs:domain rdf:resource="http://www.semanticweb.org/nina/ontologies/2016/11/erasmus#LearningOpportunityInstance"/>
        <rdfs:range rdf:resource="http://www.w3.org/2001/XMLSchema#string"/>
        <rdfs:comment>A prerequisite or entry requirement for accessing the Learning Opportunity Instance.</rdfs:comment>
        <rdfs:label>Prerequisite</rdfs:label>
    </owl:DatatypeProperty>
    


    <!-- http://www.semanticweb.org/nina/ontologies/2016/11/erasmus#qualification -->

    <owl:DatatypeProperty rdf:about="http://www.semanticweb.org/nina/ontologies/2016/11/erasmus#qualification">
        <rdfs:subPropertyOf rdf:resource="http://www.w3.org/2002/07/owl#topDataProperty"/>
        <rdfs:domain rdf:resource="http://www.semanticweb.org/nina/ontologies/2016/11/erasmus#LearningOpportunitySpecification"/>
        <rdfs:range rdf:resource="http://www.w3.org/2001/XMLSchema#string"/>
        <rdfs:comment>A qualification that can be obtained from completion of a Learning Opportunity.</rdfs:comment>
        <rdfs:label>Qualification</rdfs:label>
    </owl:DatatypeProperty>
    


    <!-- http://www.semanticweb.org/nina/ontologies/2016/11/erasmus#start -->

    <owl:DatatypeProperty rdf:about="http://www.semanticweb.org/nina/ontologies/2016/11/erasmus#start">
        <rdfs:subPropertyOf rdf:resource="http://www.w3.org/2002/07/owl#topDataProperty"/>
        <rdfs:domain rdf:resource="http://www.semanticweb.org/nina/ontologies/2016/11/erasmus#LearningOpportunityInstance"/>
        <rdfs:range rdf:resource="http://www.w3.org/2000/01/rdf-schema#Literal"/>
        <rdfs:comment>A date from which the Learning Opportunity Instance commences</rdfs:comment>
        <rdfs:label>Start</rdfs:label>
    </owl:DatatypeProperty>
    


    <!-- http://www.semanticweb.org/nina/ontologies/2016/11/erasmus#url -->

    <owl:DatatypeProperty rdf:about="http://www.semanticweb.org/nina/ontologies/2016/11/erasmus#url">
        <rdfs:domain rdf:resource="http://www.semanticweb.org/nina/ontologies/2016/11/erasmus#LearningOpportunityObject"/>
        <rdfs:range rdf:resource="http://www.w3.org/2000/01/rdf-schema#Literal"/>
        <rdfs:comment>Typically the web page of the provider or course.</rdfs:comment>
        <rdfs:label>Url</rdfs:label>
    </owl:DatatypeProperty>
    


    <!-- 
    ///////////////////////////////////////////////////////////////////////////////////////
    //
    // Classes
    //
    ///////////////////////////////////////////////////////////////////////////////////////
     -->

    


    <!-- http://www.semanticweb.org/nina/ontologies/2016/11/erasmus#CourseUnitInstance -->

    <owl:Class rdf:about="http://www.semanticweb.org/nina/ontologies/2016/11/erasmus#CourseUnitInstance">
        <rdfs:subClassOf rdf:resource="http://www.semanticweb.org/nina/ontologies/2016/11/erasmus#LearningOpportunityInstance"/>
        <owl:disjointWith rdf:resource="http://www.semanticweb.org/nina/ontologies/2016/11/erasmus#DegreeProgrammeInstance"/>
    </owl:Class>
    


    <!-- http://www.semanticweb.org/nina/ontologies/2016/11/erasmus#CourseUnitSpecification -->

    <owl:Class rdf:about="http://www.semanticweb.org/nina/ontologies/2016/11/erasmus#CourseUnitSpecification">
        <rdfs:subClassOf rdf:resource="http://www.semanticweb.org/nina/ontologies/2016/11/erasmus#LearningOpportunitySpecification"/>
        <owl:disjointWith rdf:resource="http://www.semanticweb.org/nina/ontologies/2016/11/erasmus#DegreeProgrammeSpecification"/>
    </owl:Class>
    


    <!-- http://www.semanticweb.org/nina/ontologies/2016/11/erasmus#DegreeProgrammeInstance -->

    <owl:Class rdf:about="http://www.semanticweb.org/nina/ontologies/2016/11/erasmus#DegreeProgrammeInstance">
        <rdfs:subClassOf rdf:resource="http://www.semanticweb.org/nina/ontologies/2016/11/erasmus#LearningOpportunityInstance"/>
    </owl:Class>
    


    <!-- http://www.semanticweb.org/nina/ontologies/2016/11/erasmus#DegreeProgrammeSpecification -->

    <owl:Class rdf:about="http://www.semanticweb.org/nina/ontologies/2016/11/erasmus#DegreeProgrammeSpecification">
        <rdfs:subClassOf rdf:resource="http://www.semanticweb.org/nina/ontologies/2016/11/erasmus#LearningOpportunitySpecification"/>
    </owl:Class>
    


    <!-- http://www.semanticweb.org/nina/ontologies/2016/11/erasmus#LearningOpportunityInstance -->

    <owl:Class rdf:about="http://www.semanticweb.org/nina/ontologies/2016/11/erasmus#LearningOpportunityInstance">
        <rdfs:subClassOf rdf:resource="http://www.semanticweb.org/nina/ontologies/2016/11/erasmus#LearningOpportunityObject"/>
        <rdfs:comment>A single occurrence of a learning opportunity. Unlike a Learning Opportunity Specification, a Learning
Opportunity Instance is not abstract, may be bound to particular dates or locations, and may be applied for or
participated in by learners.</rdfs:comment>
        <rdfs:label>Learning Opportunity Instance</rdfs:label>
    </owl:Class>
    


    <!-- http://www.semanticweb.org/nina/ontologies/2016/11/erasmus#LearningOpportunityObject -->

    <owl:Class rdf:about="http://www.semanticweb.org/nina/ontologies/2016/11/erasmus#LearningOpportunityObject">
        <rdfs:comment>A chance to participate in education or training.</rdfs:comment>
        <rdfs:label>Learning Opportunity Object</rdfs:label>
    </owl:Class>
    


    <!-- http://www.semanticweb.org/nina/ontologies/2016/11/erasmus#LearningOpportunityProvider -->

    <owl:Class rdf:about="http://www.semanticweb.org/nina/ontologies/2016/11/erasmus#LearningOpportunityProvider">
        <rdfs:subClassOf rdf:resource="http://www.semanticweb.org/nina/ontologies/2016/11/erasmus#LearningOpportunityObject"/>
        <rdfs:comment>An agent (person or organisation) that provides learning opportunities.</rdfs:comment>
        <rdfs:label>Learning Opportunity Provider</rdfs:label>
    </owl:Class>
    


    <!-- http://www.semanticweb.org/nina/ontologies/2016/11/erasmus#LearningOpportunitySpecification -->

    <owl:Class rdf:about="http://www.semanticweb.org/nina/ontologies/2016/11/erasmus#LearningOpportunitySpecification">
        <rdfs:subClassOf rdf:resource="http://www.semanticweb.org/nina/ontologies/2016/11/erasmus#LearningOpportunityObject"/>
        <rdfs:comment>An abstract description of a learning opportunity, consisting of information that will be consistent across
multiple instances of the learning opportunity.</rdfs:comment>
        <rdfs:label>Learning Opportunity Specification</rdfs:label>
    </owl:Class>
    


    <!-- 
    ///////////////////////////////////////////////////////////////////////////////////////
    //
    // General axioms
    //
    ///////////////////////////////////////////////////////////////////////////////////////
     -->

    <rdf:Description>
        <rdf:type rdf:resource="http://www.w3.org/2002/07/owl#AllDisjointClasses"/>
        <owl:members rdf:parseType="Collection">
            <rdf:Description rdf:about="http://www.semanticweb.org/nina/ontologies/2016/11/erasmus#LearningOpportunityInstance"/>
            <rdf:Description rdf:about="http://www.semanticweb.org/nina/ontologies/2016/11/erasmus#LearningOpportunityProvider"/>
            <rdf:Description rdf:about="http://www.semanticweb.org/nina/ontologies/2016/11/erasmus#LearningOpportunitySpecification"/>
        </owl:members>
    </rdf:Description>
</rdf:RDF>



<!-- Generated by the OWL API (version 4.2.6.20160910-2108) https://github.com/owlcs/owlapi -->

